Turned final_threads into a definition; added rule for set-predicate conversion

thys/JinjaThreads/Framework/FWSemantics.thy
@@ -96,8 +96,14 @@ by(auto intro: actions_subset.intros collect_locks'_subset_collect_locks del: su
 definition final_thread :: "('l,'t,'x,'m,'w) state \<Rightarrow> 't \<Rightarrow> bool" where
   "final_thread s t \<equiv> (case thr s t of None \<Rightarrow> False | \<lfloor>(x, ln)\<rfloor> \<Rightarrow> final x \<and> ln = no_wait_locks \<and> wset s t = None)"
 
-abbreviation final_threads :: "('l,'t,'x,'m,'w) state \<Rightarrow> 't set" 
+definition final_threads :: "('l,'t,'x,'m,'w) state \<Rightarrow> 't set" 
 where "final_threads s \<equiv> {t. final_thread s t}"
+
+lemma [iff]: "t \<in> final_threads s = final_thread s t"
+  by (simp add: final_threads_def)
+
+lemma [pred_set_conv]: "final_thread s = (\<lambda>t. t \<in> final_threads s)"
+  by simp
 
 definition mfinal :: "('l,'t,'x,'m,'w) state \<Rightarrow> bool"
 where "mfinal s \<longleftrightarrow> (\<forall>t x ln. thr s t = \<lfloor>(x, ln)\<rfloor> \<longrightarrow> final x \<and> ln = no_wait_locks \<and> wset s t = None)"
